vernac/himsg.ml
@@ -482,6 +482,8 @@ let explain_ill_formed_rec_body env sigma err names i fixenv vdefj =
      str "The return clause of the following pattern matching should be" ++
      strbrk " a coinductive type:" ++
      spc () ++ pr_lconstr_env env sigma c
+  | FixpointOnIrrelevantInductive ->
+    strbrk "Fixpoints on proof irrelevant inductive types should produce proof irrelevant values"
   in
   prt_name i ++ str " is ill-formed." ++ fnl () ++
   pr_ne_context_of (str "In environment") env sigma ++
@@ -1311,6 +1313,7 @@ let map_pguard_error f = function
 | RecCallInCasePred c -> RecCallInCasePred (f c)
 | NotGuardedForm c -> NotGuardedForm (f c)
 | ReturnPredicateNotCoInductive c -> ReturnPredicateNotCoInductive (f c)
+| FixpointOnIrrelevantInductive -> FixpointOnIrrelevantInductive
 
 let map_ptype_error f = function
 | UnboundRel n -> UnboundRel n
